atomics/general_atomics.v
@@ -1015,6 +1015,23 @@ Notation "'ATOMIC' 'TYPE' W 'OBJ' x 'INVS' Ei Eo 'WITH' x1 : t1 , x2 : t2 , x3 :
         x1 at level 0, x2 at level 0, x3 at level 0, x4 at level 0, x5 at level 0, x6 at level 0,
              S2 at level 0, r at level 0, T at level 0).
 
+Notation "'ATOMIC' 'TYPE' W 'OBJ' x 'INVS' Ei Eo 'WITH' x1 : t1 , x2 : t2 , x3 : t3 , x4 : t4 , x5 : t5 , x6 : t6 'PRE'  [ u , .. , v ] 'PROP' ( Px ; .. ; Py ) 'LOCAL' ( Lx ; .. ; Ly ) 'SEPS' ( S1x ; .. ; S1y ) '|' S2 'POST' [ tz ] 'PROP' () 'LOCAL' () 'SEP' ( SQx ; .. ; SQy )" :=
+  (mk_funspec (pair (cons u%formals .. (cons v%formals nil) ..) tz) cc_default (atomic_spec_type0 W)
+   (fun (ts: list Type) (__a : functors.MixVariantFunctor._functor (dependent_type_functor_rec ts W) mpred * mpred * invG) => let '((x1, x2, x3, x4, x5, x6), Q, inv_names) := __a in
+     PROPx (cons Px%type .. (cons Py%type nil) ..)
+     (LOCALx (cons Lx%type .. (cons Ly%type nil) ..)
+     (SEPx (cons (atomic_shift(inv_names := inv_names)(B := unit) (fun x => S2) Ei Eo (fun x _ => fold_right_sepcon (cons SQx%logic .. (cons SQy%logic nil) ..)) (fun _ => Q)) (cons S1x%logic .. (cons S1y%logic nil) ..)))))
+   (fun (ts: list Type) (__a : functors.MixVariantFunctor._functor (dependent_type_functor_rec ts W) mpred * mpred * invG) => let '((x1, x2, x3, x4, x5, x6), Q, inv_names) := __a in
+     PROP () LOCAL () (SEP (Q)))
+   (@atomic_spec_nonexpansive_pre0 _ W (cons (fun ts __a => let '(x1, x2, x3, x4, x5, x6) := __a in Px%type) .. (cons (fun ts __a => let '(x1, x2, x3, x4, x5, x6) := __a in Py%type) nil) ..)
+      (cons (fun ts __a => let '(x1, x2, x3, x4, x5, x6) := __a in Lx%type) .. (cons (fun ts __a => let '(x1, x2, x3, x4, x5, x6) := __a in Ly%type) nil) ..)
+      (cons (fun ts __a => let '(x1, x2, x3, x4, x5, x6) := __a in S1x%logic) .. (cons (fun ts __a => let '(x1, x2, x3, x4, x5, x6) := __a in S1y%logic) nil) ..)
+      (fun ts __a x => let '(x1, x2, x3, x4, x5, x6) := __a in S2) Ei Eo
+     (fun ts __a x _ => let '(x1, x2, x3, x4, x5, x6) := __a in fold_right_sepcon (cons SQx%logic .. (cons SQy%logic nil) ..)) _ _ _ _ _)
+   (atomic_spec_nonexpansive_post0 W nil _)) (at level 200, x at level 0, Ei at level 0, Eo at level 0,
+        x1 at level 0, x2 at level 0, x3 at level 0, x4 at level 0, x5 at level 0, x6 at level 0,
+             S2 at level 0).
+
 Notation "'ATOMIC' 'TYPE' W 'OBJ' x 'INVS' Ei Eo 'WITH' x1 : t1 , x2 : t2 , x3 : t3 , x4 : t4 , x5 : t5 , x6 : t6 , x7 : t7 'PRE'  [ u , .. , v ] 'PROP' ( Px ; .. ; Py ) 'LOCAL' ( Lx ; .. ; Ly ) 'SEPS' ( S1x ; .. ; S1y ) '|' S2 'POST' [ tz ] 'EX' r : T , 'PROP' () 'LOCAL' ( LQx ; .. ; LQy ) 'SEP' ( SQx ; .. ; SQy )" :=
   (mk_funspec (pair (cons u%formals .. (cons v%formals nil) ..) tz) cc_default (atomic_spec_type W T)
    (fun (ts: list Type) (__a : functors.MixVariantFunctor._functor (dependent_type_functor_rec ts W) mpred * (T -> mpred) * invG) => let '((x1, x2, x3, x4, x5, x6, x7), Q, inv_names) := __a in
